fixed rettype to type; proved step lemmas

security/Backtranslation.v
@@ -496,13 +496,54 @@ Section Backtranslation.
     Definition rettype_to_type: rettype -> type :=
       fun rt: rettype =>
         match rt with
-        | Tint8signed => Tint I8 Signed noattr
-        | Tint8unsigned => Tint I8 Unsigned noattr
-        | Tint16signed => Tint I16 Signed noattr
-        | Tint16unsigned => Tint I16 Unsigned noattr
-        | AST.Tvoid => Tvoid
+        | Tint8signed | Tint8unsigned | Tint16signed | Tint16unsigned => Tint I32 Signed noattr
+        | AST.Tvoid => Tint I32 Signed noattr
         | Tret t => typ_to_type t
         end.
+
+    (* Definition rettype_to_type: rettype -> type := *)
+    (*   fun rt: rettype => *)
+    (*     match rt with *)
+    (*     | Tint8signed => Tint I8 Signed noattr *)
+    (*     | Tint8unsigned => Tint I8 Unsigned noattr *)
+    (*     | Tint16signed => Tint I16 Signed noattr *)
+    (*     | Tint16unsigned => Tint I16 Unsigned noattr *)
+    (*     | AST.Tvoid => Tvoid *)
+    (*     | Tret t => typ_to_type t *)
+    (*     end. *)
+
+    Lemma proj_rettype_to_type_rettype_of_type_eq
+          ge evres rt res
+          (EVM: eventval_match ge evres (proj_rettype rt) res)
+      :
+      (* (rettype_of_type (rettype_to_type rt)) = rt. *)
+      proj_rettype (rettype_of_type (rettype_to_type rt)) = proj_rettype rt.
+    Proof.
+      inv EVM; destruct rt; simpl; auto.
+      destruct t; simpl in *; auto; try congruence.
+      destruct t; simpl in *; auto; try congruence.
+      destruct t; simpl in *; auto; try congruence.
+      destruct t; simpl in *; auto; try congruence.
+      unfold Tptr in *. destruct Archi.ptr64 eqn:ARCH.
+      destruct t; simpl in *; auto; try congruence.
+      destruct t; simpl in *; auto; try congruence.
+    Qed.
+
+    (* Lemma retttype_to_type_rettype_of_type_eq *)
+    (*       ge evres rt res *)
+    (*       (EVM: eventval_match ge evres (proj_rettype rt) res) *)
+    (*   : *)
+    (*   (rettype_of_type (rettype_to_type rt)) = rt. *)
+    (* Proof. *)
+    (*   inv EVM; destruct rt; simpl; auto. *)
+    (*   destruct t; simpl in *; auto; try congruence. *)
+    (*   destruct t; simpl in *; auto; try congruence. *)
+    (*   destruct t; simpl in *; auto; try congruence. *)
+    (*   destruct t; simpl in *; auto; try congruence. *)
+    (*   unfold Tptr in *. destruct Archi.ptr64 eqn:ARCH. *)
+    (*   destruct t; simpl in *; auto; try congruence. *)
+    (*   destruct t; simpl in *; auto; try congruence. *)
+    (* Qed. *)
 
     (* Wanted internal function data from signature *)
     (* Definition fun_data : Type := (typelist * type * calling_convention). *)
@@ -537,6 +578,17 @@ Section Backtranslation.
     Definition from_cl_funs_data (cl: Clight.program): funs_data :=
       let defs := Genv.genv_defs (genv_genv (globalenv cl)) in
       PTree.map_filter1 from_clgd_fun_data defs.
+
+    (* (* Return case *) *)
+    (* Definition eventval_to_expr_return (v: eventval) (rt: rettype): expr := *)
+    (*   let ty := rettype_to_type rt in *)
+    (*   match v with *)
+    (*   | EVint i => Econst_int i ty *)
+    (*   | EVlong i => Econst_long i ty *)
+    (*   | EVfloat f => Econst_float f ty *)
+    (*   | EVsingle f => Econst_single f ty *)
+    (*   | EVptr_global id ofs => ptr_of_id_ofs id ofs *)
+    (*   end. *)
 
   End CODEAUX.
 
@@ -589,6 +641,13 @@ Section Backtranslation.
           Sreturn (Some (eventval_to_expr v))
       | _ => Sskip
       end.
+
+    (* Definition code_of_return (cp cp': compartment) (v: eventval) (ik: info_kind) := *)
+    (*   match ik with *)
+    (*   | info_return sg => *)
+    (*       Sreturn (Some (eventval_to_expr_return v (sig_res sg))) *)
+    (*   | _ => Sskip *)
+    (*   end. *)
 
     Definition code_of_ievent (e: ievent): statement :=
       match e with
@@ -846,6 +905,44 @@ Section Backtranslation.
       Cop.sem_cast (Vptr b ofs) (Tpointer Tvoid noattr) (typ_to_type Tptr) m = Some (Vptr b ofs).
     Proof.
       unfold Tptr. destruct Archi.ptr64 eqn:ARCH; unfold Cop.sem_cast; simpl; rewrite ARCH; auto.
+    Qed.
+
+    Lemma sem_cast_proj_rettype
+          (ge: cgenv) evres rty res m
+          (EVM: eventval_match ge evres (proj_rettype rty) res)
+      :
+      Cop.sem_cast (eventval_to_val ge evres)
+                   (typeof (eventval_to_expr evres))
+                   (rettype_to_type rty) m
+      = Some (eventval_to_val ge evres).
+    Proof.
+      destruct rty; simpl in *.
+      { eapply eventval_match_sem_cast. eauto. erewrite eventval_match_eventval_to_val; eauto. }
+      { inv EVM; simpl; simpl_expr.
+        setoid_rewrite H2. rewrite ptr_of_id_ofs_typeof.
+        unfold Tptr in *. destruct Archi.ptr64 eqn:ARCH. congruence.
+        unfold Cop.sem_cast. simpl. rewrite ARCH. auto.
+      }
+      { inv EVM; simpl; simpl_expr.
+        setoid_rewrite H2. rewrite ptr_of_id_ofs_typeof.
+        unfold Tptr in *. destruct Archi.ptr64 eqn:ARCH. congruence.
+        unfold Cop.sem_cast. simpl. rewrite ARCH. auto.
+      }
+      { inv EVM; simpl; simpl_expr.
+        setoid_rewrite H2. rewrite ptr_of_id_ofs_typeof.
+        unfold Tptr in *. destruct Archi.ptr64 eqn:ARCH. congruence.
+        unfold Cop.sem_cast. simpl. rewrite ARCH. auto.
+      }
+      { inv EVM; simpl; simpl_expr.
+        setoid_rewrite H2. rewrite ptr_of_id_ofs_typeof.
+        unfold Tptr in *. destruct Archi.ptr64 eqn:ARCH. congruence.
+        unfold Cop.sem_cast. simpl. rewrite ARCH. auto.
+      }
+      { inv EVM; simpl; simpl_expr.
+        setoid_rewrite H2. rewrite ptr_of_id_ofs_typeof.
+        unfold Tptr in *. destruct Archi.ptr64 eqn:ARCH. congruence.
+        unfold Cop.sem_cast. simpl. rewrite ARCH. auto.
+      }
     Qed.
 
   End CODEPROP.
@@ -1187,550 +1284,84 @@ Section Backtranslation.
       }
     Qed.
 
-
     Lemma code_of_event_step_cross_call_int
-    Lemma code_of_event_step_cross_return_start
+          p f vargs k m1 m2 e le
+          (ENT: function_entry1 (globalenv p) f vargs m1 e le m2)
+      :
+      Star (Clight.semantics1 p)
+           (Callstate (Internal f) vargs k m1)
+           (nil)
+           (State f (fn_body f) k e le m2).
+    Proof.
+      subst; simpl in *. econstructor 2. eapply step_internal_function. eauto.
+      econstructor 1. auto.
+    Qed.
+
     Lemma code_of_event_step_cross_returnstate
-
-    (* TODO *)
-    Lemma code_of_event_step_call_start
-          ev
-          cp cp' id vs
-          p f k e le m
-          ge data
+          ev ik sg evres
+          p ge res optid f e le k m ty cp
           (GE: ge = globalenv p)
-          (EV: ev = Event_call cp cp' id vs)
-          (FDATA: (from_cl_funs_data p) ! id = Some data)
-          (* bt_wf *)
-          (GLOB: e ! id = None)
-          (WFARGS1: Forall (wf_eventval_env e) vs)
-          (* from_asm *)
-          b
-          (FINDB: Genv.find_symbol ge id = Some b)
-          fd
-          (FINDF: Genv.find_funct ge (Vptr b Ptrofs.zero) = Some fd)
-          (TYPEF: type_of_fundef fd = Tfunction data.(dargs) data.(dret) data.(dcc))
-          (CP1: cp = comp_of f)
-          (CP2: cp' = comp_of fd)
-          (CROSS: Genv.type_of_call ge (comp_of f) (comp_of fd) = Genv.CrossCompartmentCall)
-          (NPTR: Forall not_ptr (list_eventval_to_list_val ge vs))
-          (ALLOW: Genv.allowed_cross_call ge (comp_of f) (Vptr b Ptrofs.zero))
-          some_sig_args some_vals
-          (ESM: eventval_list_match ge vs some_sig_args some_vals)
-          (SIGARGS: data.(dargs) = (list_typ_to_typelist some_sig_args))
-      :
-        Star (Clight.semantics1 p)
-             (State f (code_of_event sid (from_cl_funs_data p) ev) k e le m)
-             (ev :: nil)
-             (Callstate fd (list_eventval_to_list_val ge vs) (Kcall None f e le k) m).
-    Proof.
-      subst; simpl. unfold code_of_call. rewrite FDATA.
-      econstructor 2.
-      3:{ rewrite E0_right. reflexivity. }
-      { eapply step_call; simpl; eauto.
-        { eapply eval_Elvalue.
-          - eapply eval_Evar_global; eauto.
-          - eapply deref_loc_reference. auto.
-        }
-        { rewrite SIGARGS. apply list_eventval_to_expr_val_eval; auto. eapply eventval_list_match_transl. eauto. }
-        red; auto.
-        unfold Genv.find_comp. setoid_rewrite FINDF.
-        eapply call_trace_cross; eauto. apply Genv.find_invert_symbol; auto.
-        rewrite SIGARGS. eapply eventval_list_match_transl; eauto.
-      }
-      econstructor 1.
-    Qed.
-
-    Lemma code_of_event_step_return
-          ev
-          cp cp' rv
-          p f k e le m
-          ge
-          (GE: ge = globalenv p)
-          (EV: ev = Event_return cp' cp rv)
-          (* bt should ensure them *)
-          (WFRV1: wf_eventval_env e rv)
-          (* asm should ensure them *)
-          (NPTR: not_ptr (eventval_to_val ge rv))
-          some_sig_ret some_val
-          (EM: eventval_match ge rv some_sig_ret some_val)
-          (RTTYP: fn_return f = typ_to_type some_sig_ret)
-          (* handle during proving *)
-          optid f' e' le' k'
-          (CONT: call_cont k = Kcall optid f' e' le' k')
-          (CP1: cp = comp_of f)
-          (CP2: cp' = comp_of f')
-          (CROSS: Genv.type_of_call ge (comp_of f') (comp_of f) = Genv.CrossCompartmentCall)
-          m'
-          (FREE: Mem.free_list m (blocks_of_env ge e) (comp_of f) = Some m')
-      :
-      Star (Clight.semantics1 p)
-           (State f (code_of_event sid (from_cl_funs_data p) ev) k e le m)
-           (ev :: nil)
-           (State f' Sskip k' e' (set_opttemp optid (eventval_to_val ge rv) le') m').
-    Proof.
-      subst; simpl. unfold code_of_return.
-      econstructor 2.
-      3:{ rewrite E0_left. reflexivity. }
-      { eapply step_return_1; simpl; eauto.
-        { eapply eventval_to_expr_val_eval; auto. eapply eventval_match_wf_eventval_ge; eauto. }
-        { rewrite RTTYP. eapply sem_cast_eventval_match. eapply eventval_match_transl; eauto. }
-      }
-      econstructor 2.
-      3:{ rewrite E0_right. reflexivity. }
-      { rewrite CONT. eapply step_returnstate; auto.
-        econstructor 2; auto. rewrite RTTYP. apply eventval_match_proj_rettype. erewrite eventval_match_eventval_to_val; eauto.
-      }
-      econstructor 1.
-    Qed.
-
-    Lemma code_of_event_step_call_internal
-          p f k e le m
-          ge
-          (GE: ge = globalenv p)
-          (* bt should ensure them *)
-          fd args f1
-          (INTERNAL: fd = Internal f1)
-          (* asm should ensure them *)
-          (* handle during proving *)
-          e1 le1 m1
-          (ENTRY: function_entry1 ge f1 args m e1 le1 m1)
-      :
-        Star (Clight.semantics1 p)
-             (Callstate fd args (Kcall None f e le k) m)
-             nil
-             (State f1 (fn_body f1) (Kcall None f e le k) e1 le1 m1).
-    Proof.
-      subst; simpl.
-      econstructor 2.
-      3:{ rewrite E0_right. reflexivity. }
-      { eapply step_internal_function; eauto. }
-      econstructor 1.
-    Qed.
-
-    Lemma code_of_event_step_vload
-          ev ik
-          ch id ofs v
-          p f k e le m ge
-          (GE: ge = globalenv p)
-          (EV: ev = Event_vload ch id ofs v)
-          fb
-          (IK: ik = info_external fb (ef_sig (EF_vload ch)))
-          fid
-          (EXT: Genv.invert_symbol ge fb = Some fid)
-          (* bt_wf *)
-          (WFENV: wf_env e id)
-          (* from_asm *)
-          b
-          (VOL: Senv.block_is_volatile ge b = true)
-          (SYMB: Genv.find_symbol ge id = Some b)
-          rv
-          (MATCH: eventval_match ge v (type_of_chunk ch) rv)
-      :
-        Star (Clight.semantics1 p)
-             (State f (code_of_ievent ge (ev, ik)) k e le m)
-             (ev :: nil)
-             (State f Sskip k e le m).
-    Proof.
-      subst; simpl in *. rewrite EXT.
-      econstructor 2.
-      3:{ rewrite E0_right. reflexivity. }
-      { eapply step_builtin.
-        { econstructor; eauto. 3: econstructor.
-          - eapply ptr_of_id_ofs_eval; eauto.
-          - destruct Archi.ptr64 eqn:ARCH.
-            + unfold ptr_of_id_ofs, Tptr. rewrite ARCH. simpl. unfold Cop.sem_cast. simpl. rewrite ARCH. eauto.
-            + unfold ptr_of_id_ofs, Tptr. rewrite ARCH. simpl. unfold Cop.sem_cast. simpl. rewrite ARCH. eauto.
-        }
-        repeat econstructor; eauto.
-      }
-      econstructor 1.
-    Qed.
-
-    Lemma code_of_event_step_vstore
-          ev
-          ch id ofs v
-          p f k e le m
-          (EV: ev = Event_vstore ch id ofs v)
-          (* bt_wf *)
-          (WFENV: wf_env e id)
-          (WFSV1: wf_eventval_env e v)
-          (* from_asm *)
-          b
-          (VOL: Senv.block_is_volatile (globalenv p) b = true)
-          (GE: Genv.find_symbol (globalenv p) id = Some b)
-          vv
-          (MATCH: eventval_match (globalenv p) v (type_of_chunk ch) (Val.load_result ch vv))
-      :
-        Star (Clight.semantics1 p)
-             (State f (code_of_event sid (from_cl_funs_data p) ev) k e le m)
-             (ev :: nil)
-             (State f Sskip k e le m).
-    Proof.
-      apply val_load_result_aux in MATCH.
-      subst; simpl in *. unfold code_of_vstore.
-      econstructor 2.
-      3:{ rewrite E0_right. reflexivity. }
-      { eapply step_builtin.
-        { econstructor; eauto.
-          { eapply ptr_of_id_ofs_eval; eauto. }
-          { destruct Archi.ptr64 eqn:ARCH.
-            - unfold ptr_of_id_ofs, Tptr. rewrite ARCH; simpl. unfold Cop.sem_cast. simpl. rewrite ARCH. eauto.
-            - unfold ptr_of_id_ofs, Tptr. rewrite ARCH; simpl. unfold Cop.sem_cast. simpl. rewrite ARCH. eauto.
-          }
-          econstructor; eauto. 3: econstructor.
-          { eapply eventval_to_expr_val_eval; auto. eapply eventval_match_wf_eventval_ge; eauto. }
-          { eapply sem_cast_eventval_match; eauto. eapply eventval_match_transl. eauto. }
-        }
-        simpl. repeat econstructor; eauto.
-      }
-      econstructor 1.
-    Qed.
-
-    Lemma code_of_event_step_annot
-          ev
-          str vs
-          p f k e le m
-          (EV: ev = Event_annot str vs)
-          (* bt_wf *)
-          (WFENV: Forall (wf_eventval_env e) vs)
-          (* from_asm *)
-          targs vargs
-          (ESM: eventval_list_match (globalenv p) vs targs vargs)
-      :
-        Star (Clight.semantics1 p)
-             (State f (code_of_event sid (from_cl_funs_data p) ev) k e le m)
-             (ev :: nil)
-             (State f Sskip k e le m).
-    Proof.
-      subst; simpl in *. unfold code_of_annot.
-      econstructor 2.
-      3:{ rewrite E0_right. reflexivity. }
-      { eapply step_builtin; simpl.
-        { eapply list_eventval_to_expr_val_eval; auto. eapply eventval_list_match_transl. eapply list_eventval_match_eventval_to_type; eauto. }
-        { repeat econstructor; eauto. eapply list_eventval_match_eventval_to_type. eapply eventval_list_match_transl; eauto. }
-      }
-      econstructor 1.
-    Qed.
-
-    Lemma code_of_event_step_call_start
-          ev
-          cp cp' id vs
-          p f k e le m
-          ge data
-          (GE: ge = globalenv p)
-          (EV: ev = Event_call cp cp' id vs)
-          (FDATA: (from_cl_funs_data p) ! id = Some data)
-          (* bt_wf *)
-          (GLOB: e ! id = None)
-          (WFARGS1: Forall (wf_eventval_env e) vs)
-          (* from_asm *)
-          b
-          (FINDB: Genv.find_symbol ge id = Some b)
-          fd
-          (FINDF: Genv.find_funct ge (Vptr b Ptrofs.zero) = Some fd)
-          (TYPEF: type_of_fundef fd = Tfunction data.(dargs) data.(dret) data.(dcc))
-          (CP1: cp = comp_of f)
-          (CP2: cp' = comp_of fd)
-          (CROSS: Genv.type_of_call ge (comp_of f) (comp_of fd) = Genv.CrossCompartmentCall)
-          (NPTR: Forall not_ptr (list_eventval_to_list_val ge vs))
-          (ALLOW: Genv.allowed_cross_call ge (comp_of f) (Vptr b Ptrofs.zero))
-          some_sig_args some_vals
-          (ESM: eventval_list_match ge vs some_sig_args some_vals)
-          (SIGARGS: data.(dargs) = (list_typ_to_typelist some_sig_args))
-      :
-        Star (Clight.semantics1 p)
-             (State f (code_of_event sid (from_cl_funs_data p) ev) k e le m)
-             (ev :: nil)
-             (Callstate fd (list_eventval_to_list_val ge vs) (Kcall None f e le k) m).
-    Proof.
-      subst; simpl. unfold code_of_call. rewrite FDATA.
-      econstructor 2.
-      3:{ rewrite E0_right. reflexivity. }
-      { eapply step_call; simpl; eauto.
-        { eapply eval_Elvalue.
-          - eapply eval_Evar_global; eauto.
-          - eapply deref_loc_reference. auto.
-        }
-        { rewrite SIGARGS. apply list_eventval_to_expr_val_eval; auto. eapply eventval_list_match_transl. eauto. }
-        red; auto.
-        unfold Genv.find_comp. setoid_rewrite FINDF.
-        eapply call_trace_cross; eauto. apply Genv.find_invert_symbol; auto.
-        rewrite SIGARGS. eapply eventval_list_match_transl; eauto.
-      }
-      econstructor 1.
-    Qed.
-
-    Lemma code_of_event_step_return
-          ev
-          cp cp' rv
-          p f k e le m
-          ge
-          (GE: ge = globalenv p)
-          (EV: ev = Event_return cp' cp rv)
-          (* bt should ensure them *)
-          (WFRV1: wf_eventval_env e rv)
-          (* asm should ensure them *)
-          (NPTR: not_ptr (eventval_to_val ge rv))
-          some_sig_ret some_val
-          (EM: eventval_match ge rv some_sig_ret some_val)
-          (RTTYP: fn_return f = typ_to_type some_sig_ret)
-          (* handle during proving *)
-          optid f' e' le' k'
-          (CONT: call_cont k = Kcall optid f' e' le' k')
-          (CP1: cp = comp_of f)
-          (CP2: cp' = comp_of f')
-          (CROSS: Genv.type_of_call ge (comp_of f') (comp_of f) = Genv.CrossCompartmentCall)
-          m'
-          (FREE: Mem.free_list m (blocks_of_env ge e) (comp_of f) = Some m')
-      :
-      Star (Clight.semantics1 p)
-           (State f (code_of_event sid (from_cl_funs_data p) ev) k e le m)
-           (ev :: nil)
-           (State f' Sskip k' e' (set_opttemp optid (eventval_to_val ge rv) le') m').
-    Proof.
-      subst; simpl. unfold code_of_return.
-      econstructor 2.
-      3:{ rewrite E0_left. reflexivity. }
-      { eapply step_return_1; simpl; eauto.
-        { eapply eventval_to_expr_val_eval; auto. eapply eventval_match_wf_eventval_ge; eauto. }
-        { rewrite RTTYP. eapply sem_cast_eventval_match. eapply eventval_match_transl; eauto. }
-      }
-      econstructor 2.
-      3:{ rewrite E0_right. reflexivity. }
-      { rewrite CONT. eapply step_returnstate; auto.
-        econstructor 2; auto. rewrite RTTYP. apply eventval_match_proj_rettype. erewrite eventval_match_eventval_to_val; eauto.
-      }
-      econstructor 1.
-    Qed.
-
-    Lemma code_of_event_step_call_internal
-          p f k e le m
-          ge
-          (GE: ge = globalenv p)
-          (* bt should ensure them *)
-          fd args f1
-          (INTERNAL: fd = Internal f1)
-          (* asm should ensure them *)
-          (* handle during proving *)
-          e1 le1 m1
-          (ENTRY: function_entry1 ge f1 args m e1 le1 m1)
-      :
-        Star (Clight.semantics1 p)
-             (Callstate fd args (Kcall None f e le k) m)
-             nil
-             (State f1 (fn_body f1) (Kcall None f e le k) e1 le1 m1).
-    Proof.
-      subst; simpl.
-      econstructor 2.
-      3:{ rewrite E0_right. reflexivity. }
-      { eapply step_internal_function; eauto. }
-      econstructor 1.
-    Qed.
-
-    Lemma code_of_event_step_call_external_cross
-          p m
-          ge
-          (GE: ge = globalenv p)
-          (* bt should ensure them *)
-          fd k args ef targs tres cconv
-          (EXTERNAL: fd = External ef targs tres cconv)
-          (* asm should ensure them *)
-          sev
-          vres m1
-          (SEM: external_call ef ge (call_comp k) args m (sev :: nil) vres m1)
-          (* handle during proving *)
-          sname sargs svr
-          (SYSEV: sev = Event_syscall sname sargs svr)
-      :
-        Star (Clight.semantics1 p)
-             (Callstate fd args k m)
-             (sev :: nil)
-             (Returnstate vres k m1 (rettype_of_type tres) (comp_of ef)).
-    Proof.
-      subst; simpl.
-      econstructor 2.
-      3:{ rewrite E0_right. reflexivity. }
-      { eapply step_external_function; eauto. }
-      econstructor 1.
-    Qed.
-
-    Lemma code_of_event_step_return_external_cross
-          p m
-          ge
-          (GE: ge = globalenv p)
-          ev rv f cp
-          (EV: ev = Event_return (comp_of f) cp rv)
-          (* bt should ensure them *)
-          (* asm should ensure them *)
-          vres optid e le k ty
+          (EV: ev = Event_return (comp_of f) cp evres)
+          (IK: ik = info_return sg)
           (CROSS: Genv.type_of_call ge (comp_of f) cp = Genv.CrossCompartmentCall)
-          (NPTR: not_ptr vres)
-          (EM: eventval_match ge rv (proj_rettype ty) vres)
-          (* handle during proving *)
+          (EVM: eventval_match ge evres (proj_rettype (sig_res sg)) res)
+          (NPTR: not_ptr res)
+          (RETTY: ty = sig_res sg)
       :
-        Star (Clight.semantics1 p)
-             (Returnstate vres (Kcall optid f e le k) m ty cp)
-             (ev :: nil)
-             (State f Sskip k e (set_opttemp optid vres le) m).
+      Star (Clight.semantics1 p)
+           (Returnstate res (Kcall optid f e le k) m ty cp)
+           (ev :: nil)
+           (State f Sskip k e (set_opttemp optid res le) m).
     Proof.
-      subst; simpl.
-      econstructor 2.
-      3:{ rewrite E0_right. reflexivity. }
+      subst; simpl. econstructor 2.
       { eapply step_returnstate; eauto. econstructor 2; eauto. }
-      econstructor 1.
+      econstructor 1. auto.
     Qed.
 
+    Lemma code_of_event_step_cross_return_code
+          ev ik
+          p f k e le m ge cp
+          (CP: cp = comp_of f)
+          (GE: ge = globalenv p)
+          cp_c evres
+          (EV: ev = Event_return cp_c cp evres)
+          (WF: wf_eventval_env e evres)
+          sg
+          (IK: ik = info_return sg)
+          (CROSS: Genv.type_of_call ge cp_c cp = Genv.CrossCompartmentCall)
+          optid f_c e_c le_c k_c
+          (CONT: call_cont k = Kcall optid f_c e_c le_c k_c)
+          (CPC: cp_c = comp_of f_c)
+          res
+          (EVM: eventval_match ge evres (proj_rettype (sig_res sg)) res)
+          (NPTR: not_ptr res)
+          (TY: fn_return f = rettype_to_type (sig_res sg))
+          m'
+          (FREE: Mem.free_list m (blocks_of_env ge e) cp = Some m')
+      :
+      Star (Clight.semantics1 p)
+           (State f (code_of_ievent ge (ev, ik)) k e le m)
+           (ev :: nil)
+           (State f_c Sskip k_c e_c (set_opttemp optid res le_c) m').
+    Proof.
+      subst; simpl. exploit eventval_match_eventval_to_val. eapply EVM. intros RES.
+      econstructor 2.
+      { eapply step_return_1; eauto.
+        { eapply eventval_to_expr_val_eval; auto. eapply eventval_match_wf_eventval_ge; eauto. }
+        { rewrite TY. eapply sem_cast_proj_rettype. eauto. }
+      }
+      econstructor 2.
+      { rewrite CONT. eapply step_returnstate.
+        { subst res. auto. }
+        { econstructor 2; auto. rewrite TY. erewrite proj_rettype_to_type_rettype_of_type_eq.
+          2: eauto. subst res; eauto.
+        }
+      }
+      { subst res. econstructor 1. }
+      all: eauto.
+    Qed.
 
     (* TODO *)
-    Lemma code_of_event_step_call_external_intra
-          ev
-          name args rv
-          p f k e le m
-          ge data
-          (GE: ge = globalenv p)
-          (EV: ev = Event_syscall name args rv)
-          (* start call *)
-          id
-          (ID: sid name = Some (sys_external id))
-          (FDATA: (from_cl_funs_data p) ! id = Some data)
-          (* bt_wf *)
-          (GLOB: e ! id = None)
-          (WFARGS1: Forall (wf_eventval_env e) args)
-          (* (WFARGS2: Forall (wf_eventval_ge ge) args) *)
-          (* from_asm *)
-          b
-          (FINDB: Genv.find_symbol ge id = Some b)
-          (ALLOW: Genv.allowed_call ge (comp_of f) (Vptr b Ptrofs.zero))
-          fd
-          (FINDF: Genv.find_funct ge (Vptr b Ptrofs.zero) = Some fd)
-          (TYPEF: type_of_fundef fd = Tfunction data.(dargs) data.(dret) data.(dcc))
-          cp cp'
-          (CP1: cp = comp_of f)
-          (CP2: cp' = comp_of fd)
-          (INTRA: Genv.type_of_call ge (comp_of f) (comp_of fd) <> Genv.CrossCompartmentCall)
-          (* invoke syscall *)
-          ef
-          (* name' cp'' sg *)
-          (* (EF: ef = EF_external name' cp'' sg) *)
-          (EXTERNAL: fd = External ef data.(dargs) data.(dret) data.(dcc))
-          srv m'
-          (SEM: external_call ef ge cp (list_eventval_to_list_val (globalenv p) args) m (ev :: nil) srv m')
-          (* returnstate *)
-          (* conditions for argument types - might need extra semantics for EF_external *)
-          (* (TYARGS: data.(dargs) = (list_eventval_to_typelist args)) *)
-          some_sig_args some_vals
-          (ESM: eventval_list_match ge args some_sig_args some_vals)
-          (SIGARGS: data.(dargs) = (list_typ_to_typelist some_sig_args))
-      :
-        Star (Clight.semantics1 p)
-             (State f (code_of_event sid (from_cl_funs_data p) ev) k e le m)
-             (ev :: nil)
-             (State f Sskip k e le m').
-    Proof.
-      subst; simpl. unfold code_of_syscall. rewrite ID. rewrite FDATA.
-      econstructor 2.
-      3:{ rewrite E0_left. reflexivity. }
-      { eapply step_call. simpl; eauto.
-        { eapply eval_Elvalue.
-          - eapply eval_Evar_global; eauto.
-          - eapply deref_loc_reference. auto.
-        }
-        (* { rewrite TYARGS. eapply list_eventval_to_expr_val_eval2; auto. } *)
-        { rewrite SIGARGS. instantiate (1:=list_eventval_to_list_val (globalenv p) args).
-          eapply list_eventval_to_expr_val_eval_typs; auto. eapply eventval_list_match_transl_val; eauto.
-        }
-        all: simpl in *; eauto.
-        { unfold Genv.find_comp. unfold Genv.find_funct.
-          rewrite pred_dec_true; auto. rewrite pred_dec_true in FINDF; auto.
-          rewrite FINDF. intros. exfalso. apply INTRA. auto.
-        }
-        { econstructor 1. unfold Genv.find_comp. unfold Genv.find_funct.
-          rewrite pred_dec_true; auto. rewrite pred_dec_true in FINDF; auto.
-          rewrite FINDF. intros H. apply INTRA. auto.
-        }
-      }
-      econstructor 2.
-      3:{ rewrite E0_right. reflexivity. }
-      { eapply step_external_function. eauto. }
-      econstructor 2.
-      3:{ rewrite E0_right. reflexivity. }
-      { eapply step_returnstate. intro. exfalso. apply INTRA. auto.
-        econstructor 1. intros H. apply INTRA. auto.
-      }
-      econstructor 1.
-    Qed.
-
-    Lemma code_of_event_step_builtin
-          ev
-          name args rv
-          p f k e le m
-          ge
-          (GE: ge = globalenv p)
-          (EV: ev = Event_syscall name args rv)
-          name' sg
-          (ID: sid name = Some (sys_builtin name' sg))
-          (* bt_wf *)
-          (WFARGS: Forall (wf_eventval_env e) args)
-          (* from_asm *)
-          (* invoke syscall *)
-          ef
-          (EF: ef = EF_builtin name' sg)
-          srv m'
-          (SEM: external_call ef ge (comp_of f) (list_eventval_to_list_val (globalenv p) args) m (ev :: nil) srv m')
-          (* conditions for argument types - might need extra semantics for EF_external *)
-          (* (TYARGS: data.(dargs) = (list_eventval_to_typelist args)) *)
-          some_sig_args some_vals
-          (ESM: eventval_list_match ge args some_sig_args some_vals)
-          (SIGARGS: sg.(sig_args) = (some_sig_args))
-      :
-        Star (Clight.semantics1 p)
-             (State f (code_of_event sid (from_cl_funs_data p) ev) k e le m)
-             (ev :: nil)
-             (State f Sskip k e le m').
-    Proof.
-      subst; simpl. unfold code_of_syscall. rewrite ID.
-      econstructor 2.
-      3:{ rewrite E0_right. reflexivity. }
-      { eapply step_builtin; simpl; eauto. eapply list_eventval_to_expr_val_eval_typs; auto. eapply eventval_list_match_transl_val; eauto. }
-      econstructor 1.
-    Qed.
-
-    Lemma code_of_event_step_inline
-          ev
-          name args rv
-          p f k e le m
-          ge
-          (GE: ge = globalenv p)
-          (EV: ev = Event_syscall name args rv)
-          txt sg strs
-          (ID: sid name = Some (sys_inline txt sg strs))
-          (* bt_wf *)
-          (WFARGS: Forall (wf_eventval_env e) args)
-          (* from_asm *)
-          (* invoke syscall *)
-          ef
-          (EF: ef = EF_inline_asm txt sg strs)
-          srv m'
-          (SEM: external_call ef ge (comp_of f) (list_eventval_to_list_val (globalenv p) args) m (ev :: nil) srv m')
-          (* conditions for argument types - might need extra semantics for EF_external *)
-          (* (TYARGS: data.(dargs) = (list_eventval_to_typelist args)) *)
-          some_sig_args some_vals
-          (ESM: eventval_list_match ge args some_sig_args some_vals)
-          (SIGARGS: sg.(sig_args) = (some_sig_args))
-      :
-        Star (Clight.semantics1 p)
-             (State f (code_of_event sid (from_cl_funs_data p) ev) k e le m)
-             (ev :: nil)
-             (State f Sskip k e le m').
-    Proof.
-      subst; simpl. unfold code_of_syscall. rewrite ID.
-      econstructor 2.
-      3:{ rewrite E0_right. reflexivity. }
-      { eapply step_builtin; simpl; eauto. eapply list_eventval_to_expr_val_eval_typs; auto. eapply eventval_list_match_transl_val; eauto. }
-      econstructor 1.
-    Qed.
-
   End STEPPROP.
 
 
